\documentclass[../main.tex]{subfile}

\begin{document}

\topictitle{Binomial Expansion}

\sectitle{Definitions}

\vspace{-0.8em}
\begin{center}
The factorial $n! \equiv n \times (n - 1) \times (n - 2) \times \cdots \times 3 \times 2 \times 1$.

The falling factorial $n^{\underline{k}} \equiv n \times (n - 1) \times (n - 2) \times \cdots \times (n - (k - 2)) \times (n - (k - 1))$. It has $k$ terms.

$\boxed{0! = n^{\underline{0}} = 1}$

The choose function \formulaBookBox{$\displaystyle ^n C_r \equiv \binom{n}{r} \equiv \frac{n!}{r! (n - r)!}$}
\end{center}

\sectitle{Expansions}

\vspace{-0.8em}
\begin{center}
	For a natural number $n$, the expansion of $(a + b)^n$ is
\begin{empheq}[box=\formulaBookBox]{align*}
	\displaystyle a^n + n a^{n - 1} b + \binom{n}{2} a^{n - 2} b^2 + \cdots \binom{n}{r} a^{n - r} b^r + \cdots b^n
\end{empheq}

In general, $\boxed{\displaystyle (a + b)^n = \sum_{r = 0}^n \binom{n}{r} a^{n - r} b^r}\ \constraint{n \in \mathbb{N}}$

That's true if $n$ is a natural number, but there is a version that works for all real numbers. For an expression $(a + bx)^n$, it should first be normalised to $a^n (1 + \frac{b}{a} x)^n$. Let $y = \frac{b}{a} x$. Then the expansion of $(1 + y)^n$ is given by
\begin{empheq}[box=\formulaBookBox]{align*}
	\displaystyle
	(1 + y)^n \equiv
	1 + ny + \frac{n (n - 1)}{2!} y^2 + \frac{n (n - 1) (n - 2)}{3!} y^3 + \cdots + \frac{n (n - 1) (n - 2) \cdots (n - (r - 1))}{r!} y^r + \cdots
\end{empheq}

In general, \rememberBox{$\displaystyle (a + bx)^n = a^n \sum_{r = 0}^\infty \frac{n^{\underline{r}}}{r!} \left(\frac{b}{a} x\right)^r$}\ $\constraint{n \in \mathbb{R}}$
\end{center}

\end{document}
